dataplane/Examples/Tmap_op.thy
@@ -12,4 +12,33 @@ definition \<open>tmap_op ip op os f = builder_op False {|ip|} {|op|} os (\<lamb
     |}
    )\<close>
 
+lemma is_Inl_alt: "is_Inl x = (\<exists>x'. x = Inl x')"
+  by(cases x; simp)
+
+lemma is_Inr_alt: "is_Inr x \<Longrightarrow> \<exists>x'. x = Inr x'"
+  by(cases x; simp)
+
+lemma step_tmap_op_elim: 
+  assumes "step io (tmap_op ip op os f) op'"
+  obtains x where "io = Inp None (Inl (Inl x))" "op' = \<oslash>" |
+        x where "io = Inp None (Inr x)" "op' = \<oslash>" |
+        fa where "io = Inp None (Inl (Inr fa))" "\<not> initia os" "op' = tmap_op ip op (os\<lparr>front := fa, initia := True, nfron := True\<rparr>) f" |
+        x where "io = Inp (Some ip) (Inl x)" "initia os" "op' = \<oslash>" |
+        p d t where "io = Inp (Some ip) (Inr (d, t))" "initia os" "op' = tmap_op ip op (consumes os p t d) f" |
+        os' st where "io = Out None (Inl (Inl st))" "initia os" "has_progress os" "(os', st) = obtain_progress os" "op' = tmap_op ip op os' f" |
+        p x xs where "io = Out (Some op) (Inr x)" "initia os" "outpu os op = x # xs" "op' = tmap_op ip op (os\<lparr>outpu := (outpu os)(p := xs)\<rparr>) f" |
+        os' where "io = Tau" "initia os" "\<exists>p. ocaps os p \<noteq> []" 
+            "os' |\<in>| {|let result = map (\<lambda>(d, y). (f (de1 os d), y)) (input os ip); os = trace STR ''producing from tmap op'' (produces os (map (\<lambda>(d, t). (en2 os d, Cap t op)) result))
+             in Let (drop_caps os (concat (map (\<lambda>p. map (\<lambda>t. Cap t p) (ocaps os p)) enum_class.enum))) (input_update (\<lambda>_ p. []))|}"
+             "op' = tmap_op ip op os' f"
+  using assms
+  apply -
+  unfolding tmap_op_def
+  apply(drule step_builder_op_elim; (simp only: is_Inr_alt is_Inl_alt tmap_op_def[symmetric])?)
+      apply (metis (lifting) is_Inl.simps(2) is_Inr.simps(2) reassoc.cases sum.sel(1))
+     apply(blast)+
+  done
+
+
+
 end
